# Perfect Secrecy of the One-time Pad

## Construction

!!! info "Definition of \_âŠ•\_" 

    \_âŠ•\_ is bitwise XOR: $\quad 0 âŠ• 0 = 0, \quad 0 âŠ• 1 = 1, \quad 1 âŠ• 0 = 1, \quad 1 âŠ• 1 = 0$.

    For n-bit strings $\; a = aâ‚ â‹¯ a_n$, $\; b = bâ‚ â‹¯ b_n$ , let $\; a âŠ• b = aâ‚ âŠ• bâ‚ â‹¯ a_n âŠ• b_n$.

??? info "Cayley table of \_âŠ•\_"

    âŠ• | 0 | 1
    --| --| --
    0 | 0 | 1
    1 | 1 | 0


!!! note "An important property of \_âŠ•\_"

    $a âŠ• b = c â‡” a = b âŠ• c$, for all $a$, $b$, $c$. 


Fix an integer $n > 0$. 

Let $â„³$ be the *message space* , $ğ’¦$ the *key space*, and $ğ’$ the *ciphertext space*.

Assume $â„³$, $ğ’¦$, $ğ’$ all equal $\{0, 1\}^n$.

+  **Gen** (key-generation algorithm) choose key from *uniform distribution* over $ğ’¦$.

+  **Enc** (encryption algorithm) given $k âˆˆ ğ’¦$, $m âˆˆ â„³$,  output ciphertext $c = k âŠ• m$.

+  **Dec** (decryption algorithm) given $k âˆˆ ğ’¦$, $c âˆˆ ğ’$, output message $m = k âŠ• c$.

## Perfect Secrecy Theorem

!!! note "Theorem 2.9 (Katz & Lindell, 2ed)"

    The one-time pad encryption scheme is perfectly secret.

??? note "Proof of Theorem 2.9 âœï¸"

    + Let $C$ and $M$ be r.v.s from arbitrary, fixed distributions over $â„³$ and $ğ’$, resp.
    + Let $K$ be a r.v. from the uniform distribution over $ğ’¦$.

    !!! note "**Goal** ğŸ¥…"

        If $m âˆˆ â„³$, $c âˆˆ ğ’$ and $â„™(C = c) > 0$, then $â„™ (M = m \; | \; C = c) = â„™(M = m)$.

    We first show what amounts to "$C$ is uniform if $K$ is uniform, regardless of $M$."
    
    Compute $â„™(C = c \; | \; M = m )$ for arbitrary $c âˆˆ ğ’$ and $m âˆˆ â„³$:
    \\[â„™ (C = c \; | \; M = m) = â„™ (\mathrm{Enc}_k (m) = c) = â„™(k âŠ• m = c)= â„™(k = m âŠ• c)= 2^{-n},\\]

    since $k$ is chosen from a uniform distribution over the set $ğ’¦$ of $n$-bit strings.

    For $c âˆˆ ğ’$,

    \\[â„™ (C = c) = âˆ‘\_{m âˆˆ â„³} â„™ (C = c \; | \; M = m) Â· â„™(M = m) = 2^{-n} âˆ‘\_{m âˆˆ â„³} â„™(M = m) = 2^{-n}.\\] 

    Finally, by Bayes' Theorem,

    \begin{align*}
    â„™(M = m \; | \; C = c) &= \frac{â„™(C = c \; | \; M = m) Â· â„™(M = m)}{â„™(C = c)}\\
                           &= \frac{2^{-n} Â· â„™(M = m)}{2^{-n}} = â„™(M = m).
    \end{align*}

    âˆ


